JSON -> IR

theories/Jexp.v
@@ -14,44 +14,44 @@ Export
 Open Scope parser_scope.
 
 Inductive jexp :=
-  Jexp__Const  : json                             -> jexp
+  Jexp__Const  : IR                               -> jexp
 | Jexp__Array  : list jexp                        -> jexp
 | Jexp__Object : list (string * jexp)             -> jexp
-| Jexp__Ref    : labelT -> jpath -> (json -> json)   -> jexp.
+| Jexp__Ref    : labelT -> jpath -> (IR -> IR)       -> jexp.
 
-Definition nth_weak (fp : json -> option json) (n : nat) (j : json)
-  : option json :=
+Definition nth_weak (fp : IR -> option IR) (n : nat) (j : IR)
+  : option IR :=
   if j is JSON__Array l then
     get_nth n j >>= fp <|>
     last (map Some $ pick_some (map fp l)) None
   else None.
 
-Fixpoint jget_weak (p : jpath) (j : json) : option json :=
+Fixpoint jget_weak (p : jpath) (j : IR) : option IR :=
   match p with
   | Jpath__This        => Some j
   | Jpath__Array  n p' => nth_weak (jget_weak p') n j
   | Jpath__Object s p' => get_json' s j >>= jget_weak p'
   end.
 
-Example tget_strong (l : labelT) (p : jpath) (t : traceT) : json :=
+Example tget_strong (l : labelT) (p : jpath) (t : traceT) : IR :=
   odflt JSON__Null $ packet__payload <$> get l t >>= jget p.
 
-Definition tget_weak' (jget : jpath -> json -> option json)
-           (l : labelT) (p : jpath) (t : traceT) : json :=
+Definition tget_weak' (jget : jpath -> IR -> option IR)
+           (l : labelT) (p : jpath) (t : traceT) : IR :=
   odflt (last (pick_some $ map (jget p ∘ packet__payload ∘ snd) t) JSON__Null) $
         packet__payload <$> get l t >>= jget p.
 
-Definition tget_weak : labelT -> jpath -> traceT -> json := tget_weak' jget_weak.
+Definition tget_weak : labelT -> jpath -> traceT -> IR := tget_weak' jget_weak.
 
-Fixpoint jexp_to_json' (tget : labelT -> jpath -> traceT -> json)
-         (t : traceT) (e : jexp) : json :=
+Fixpoint jexp_to_IR' (tget : labelT -> jpath -> traceT -> IR)
+         (t : traceT) (e : jexp) : IR :=
   match e with
   | Jexp__Const  j => j
-  | Jexp__Array  l => JSON__Array  $ map     (jexp_to_json' tget t) l
-  | Jexp__Object m => JSON__Object $ map_snd (jexp_to_json' tget t) m
+  | Jexp__Array  l => JSON__Array  $ map     (jexp_to_IR' tget t) l
+  | Jexp__Object m => JSON__Object $ map_snd (jexp_to_IR' tget t) m
   | Jexp__Ref  l p f => f $ tget l p t
   end.
 
-Example jexp_to_json_strong : traceT -> jexp -> json := jexp_to_json' tget_strong.
+Example jexp_to_IR_strong : traceT -> jexp -> IR := jexp_to_IR' tget_strong.
 
-Definition jexp_to_json_weak : traceT -> jexp -> json := jexp_to_json' tget_weak.
+Definition jexp_to_IR_weak : traceT -> jexp -> IR := jexp_to_IR' tget_weak.
